WIP

src/KnotSim.v
@@ -8,7 +8,7 @@ Require Import Program.
 Export ITreeNotations.
 
 From Fairness Require Export ITreeLib FairBeh NatStructs.
-From Fairness Require Export Mod ModSimGStutter Concurrency.
+From Fairness Require Export Mod ModSimStutter Concurrency.
 From Fairness Require Import pind PCM World.
 
 Set Implicit Arguments.
@@ -40,12 +40,11 @@ Section KSIM.
        (@imap ident_tgt wf_tgt) *
        state_src *
        state_tgt *
-       wf_stt.(T) *
        URA.car)%type.
 
-  Definition to_kshared (shr: shared state_src state_tgt _ident_src _ident_tgt wf_src wf_tgt wf_stt): kshared :=
-    let '(ths, tht, im_src, im_tgt, st_src, st_tgt, o, r_shared) := shr in
-    (im_src, im_tgt, st_src, st_tgt, o, r_shared).
+  Definition to_kshared (shr: shared state_src state_tgt _ident_src _ident_tgt wf_src wf_tgt): kshared :=
+    let '(ths, im_src, im_tgt, st_src, st_tgt, r_shared) := shr in
+    (im_src, im_tgt, st_src, st_tgt, r_shared).
 
   Definition threads2 _id ev R := Th.t (prod bool (@thread _id ev R)).
   Notation threads_src1 R0 := (threads _ident_src (sE state_src) R0).
@@ -53,11 +52,11 @@ Section KSIM.
   Notation threads_tgt R1 := (threads _ident_tgt (sE state_tgt) R1).
 
   Variant __sim_knot R0 R1 (RR: R0 -> R1 -> Prop)
-          (sim_knot: threads_src2 R0 -> threads_tgt R1 -> thread_id -> local_resources -> bool -> bool -> (prod bool (itree srcE R0)) -> (itree tgtE R1) -> kshared -> Prop)
-          (_sim_knot: threads_src2 R0 -> threads_tgt R1 -> thread_id -> local_resources -> bool -> bool -> (prod bool (itree srcE R0)) -> (itree tgtE R1) -> kshared -> Prop)
+          (sim_knot: threads_src2 R0 -> threads_tgt R1 -> thread_id -> local_resources -> bool -> bool -> (prod bool (itree srcE R0)) -> (itree tgtE R1) -> kshared -> wf_stt.(T) -> Prop)
+          (_sim_knot: threads_src2 R0 -> threads_tgt R1 -> thread_id -> local_resources -> bool -> bool -> (prod bool (itree srcE R0)) -> (itree tgtE R1) -> kshared -> wf_stt.(T) -> Prop)
           (thsl: threads_src2 R0) (thsr: threads_tgt R1)
     :
-    thread_id -> local_resources -> bool -> bool -> (prod bool (itree srcE R0)) -> itree tgtE R1 -> kshared -> Prop :=
+    thread_id -> local_resources -> bool -> bool -> (prod bool (itree srcE R0)) -> itree tgtE R1 -> kshared -> wf_stt.(T) -> Prop :=
     | ksim_ret_term
         tid f_src f_tgt
         sf r_src r_tgt
@@ -70,7 +69,7 @@ Section KSIM.
       __sim_knot RR sim_knot _sim_knot thsl thsr tid rs_local f_src f_tgt
                  (sf, Ret r_src)
                  (Ret r_tgt)
-                 (im_src, im_tgt, st_src, st_tgt, o, r_kshared)
+                 (im_src, im_tgt, st_src, st_tgt, r_kshared) o
 
     | ksim_ret_cont
         tid f_src f_tgt
@@ -98,7 +97,7 @@ Section KSIM.
                                             ps pt
                                             (b, Vis (inl1 (inr1 Yield)) (fun _ => th_src))
                                             (th_tgt)
-                                            (im_src, im_tgt0, st_src, st_tgt, o0, r_shared0)))) /\
+                                            (im_src, im_tgt0, st_src, st_tgt, r_shared0) o0))) /\
                     ((b = false) ->
                      (forall im_tgt0
                         (FAIR: fair_update im_tgt im_tgt0 (sum_fmap_l (tids_fmap tid0 (key_set thsr0)))),
@@ -109,12 +108,12 @@ Section KSIM.
                                               ps pt
                                               (b, th_src)
                                               th_tgt
-                                              (im_src0, im_tgt0, st_src, st_tgt, o0, r_shared0))))))
+                                              (im_src0, im_tgt0, st_src, st_tgt, r_shared0) o0)))))
       :
       __sim_knot RR sim_knot _sim_knot thsl thsr tid rs_local f_src f_tgt
                  (sf, Ret r_src)
                  (Ret r_tgt)
-                 (im_src, im_tgt, st_src, st_tgt, o, r_kshared)
+                 (im_src, im_tgt, st_src, st_tgt, r_kshared) o
 
     | ksim_sync
         tid f_src f_tgt
@@ -140,7 +139,7 @@ Section KSIM.
                                                  ps pt
                                                  (b, Vis (inl1 (inr1 Yield)) (fun _ => th_src))
                                                  (th_tgt)
-                                                 (im_src, im_tgt0, st_src, st_tgt, o0, r_shared0))) /\
+                                                 (im_src, im_tgt0, st_src, st_tgt, r_shared0) o0)) /\
                     ((b = false) ->
                      (forall im_tgt0 (FAIR: fair_update im_tgt im_tgt0 (sum_fmap_l (tids_fmap tid0 (key_set thsr1)))),
                        exists im_src0 o0,
@@ -151,12 +150,12 @@ Section KSIM.
                                               ps pt
                                               (b, th_src)
                                               th_tgt
-                                              (im_src0, im_tgt0, st_src, st_tgt, o0, r_shared0))))))
+                                              (im_src0, im_tgt0, st_src, st_tgt, r_shared0) o0)))))
       :
       __sim_knot RR sim_knot _sim_knot thsl thsr tid rs_local f_src f_tgt
                  (sf, Vis (inl1 (inr1 Yield)) ktr_src)
                  (Vis (inl1 (inr1 Yield)) ktr_tgt)
-                 (im_src, im_tgt, st_src, st_tgt, o, r_kshared)
+                 (im_src, im_tgt, st_src, st_tgt, r_kshared) o
 
     | ksim_yieldL
         tid f_src f_tgt
@@ -168,12 +167,12 @@ Section KSIM.
               (_sim_knot thsl thsr tid rs_local true f_tgt
                          (false, ktr_src tt)
                          itr_tgt
-                         (im_src0, im_tgt, st_src, st_tgt, o0, r_kshared)))
+                         (im_src0, im_tgt, st_src, st_tgt, r_kshared) o0))
       :
       __sim_knot RR sim_knot _sim_knot thsl thsr tid rs_local f_src f_tgt
                  (sf, Vis (inl1 (inr1 Yield)) ktr_src)
                  (itr_tgt)
-                 (im_src, im_tgt, st_src, st_tgt, o, r_kshared)
+                 (im_src, im_tgt, st_src, st_tgt, r_kshared) o
 
     | ksim_tauL
         tid f_src f_tgt
@@ -183,12 +182,12 @@ Section KSIM.
         (KSIM: _sim_knot thsl thsr tid rs_local true f_tgt
                          (sf, itr_src)
                          itr_tgt
-                         (im_src, im_tgt, st_src, st_tgt, o0, r_kshared))
+                         (im_src, im_tgt, st_src, st_tgt, r_kshared) o0)
       :
       __sim_knot RR sim_knot _sim_knot thsl thsr tid rs_local f_src f_tgt
                  (sf, Tau itr_src)
                  (itr_tgt)
-                 (im_src, im_tgt, st_src, st_tgt, o, r_kshared)
+                 (im_src, im_tgt, st_src, st_tgt, r_kshared) o
     | ksim_chooseL
         tid f_src f_tgt
         sf X ktr_src itr_tgt
@@ -197,12 +196,12 @@ Section KSIM.
         (KSIM: exists x, _sim_knot thsl thsr tid rs_local true f_tgt
                               (sf, ktr_src x)
                               itr_tgt
-                              (im_src, im_tgt, st_src, st_tgt, o0, r_kshared))
+                              (im_src, im_tgt, st_src, st_tgt, r_kshared) o0)
       :
       __sim_knot RR sim_knot _sim_knot thsl thsr tid rs_local f_src f_tgt
                  (sf, Vis (inl1 (inl1 (Choose X))) ktr_src)
                  (itr_tgt)
-                 (im_src, im_tgt, st_src, st_tgt, o, r_kshared)
+                 (im_src, im_tgt, st_src, st_tgt, r_kshared) o
     | ksim_putL
         tid f_src f_tgt
         sf st_src0 ktr_src itr_tgt
@@ -211,12 +210,12 @@ Section KSIM.
         (KSIM: _sim_knot thsl thsr tid rs_local true f_tgt
                          (sf, ktr_src tt)
                          itr_tgt
-                         (im_src, im_tgt, st_src0, st_tgt, o0, r_kshared))
+                         (im_src, im_tgt, st_src0, st_tgt, r_kshared) o0)
       :
       __sim_knot RR sim_knot _sim_knot thsl thsr tid rs_local f_src f_tgt
                  (sf, Vis (inr1 (Mod.Put st_src0)) ktr_src)
                  (itr_tgt)
-                 (im_src, im_tgt, st_src, st_tgt, o, r_kshared)
+                 (im_src, im_tgt, st_src, st_tgt, r_kshared) o
     | ksim_getL
         tid f_src f_tgt
         sf ktr_src itr_tgt
@@ -225,12 +224,12 @@ Section KSIM.
         (KSIM: _sim_knot thsl thsr tid rs_local true f_tgt
                          (sf, ktr_src st_src)
                          itr_tgt
-                         (im_src, im_tgt, st_src, st_tgt, o0, r_kshared))
+                         (im_src, im_tgt, st_src, st_tgt, r_kshared) o0)
       :
       __sim_knot RR sim_knot _sim_knot thsl thsr tid rs_local f_src f_tgt
                  (sf, Vis (inr1 (@Mod.Get _)) ktr_src)
                  (itr_tgt)
-                 (im_src, im_tgt, st_src, st_tgt, o, r_kshared)
+                 (im_src, im_tgt, st_src, st_tgt, r_kshared) o
     | ksim_tidL
         tid f_src f_tgt
         sf ktr_src itr_tgt
@@ -239,12 +238,12 @@ Section KSIM.
         (KSIM: _sim_knot thsl thsr tid rs_local true f_tgt
                          (sf, ktr_src tid)
                          itr_tgt
-                         (im_src, im_tgt, st_src, st_tgt, o0, r_kshared))
+                         (im_src, im_tgt, st_src, st_tgt, r_kshared) o0)
       :
       __sim_knot RR sim_knot _sim_knot thsl thsr tid rs_local f_src f_tgt
                  (sf, Vis (inl1 (inr1 GetTid)) ktr_src)
                  (itr_tgt)
-                 (im_src, im_tgt, st_src, st_tgt, o, r_kshared)
+                 (im_src, im_tgt, st_src, st_tgt, r_kshared) o
     | ksim_UB
         tid f_src f_tgt
         sf ktr_src itr_tgt
@@ -254,7 +253,7 @@ Section KSIM.
       __sim_knot RR sim_knot _sim_knot thsl thsr tid rs_local f_src f_tgt
                  (sf, Vis (inl1 (inl1 Undefined)) ktr_src)
                  (itr_tgt)
-                 (im_src, im_tgt, st_src, st_tgt, o, r_kshared)
+                 (im_src, im_tgt, st_src, st_tgt, r_kshared) o
     | ksim_fairL
         tid f_src f_tgt
         sf fm ktr_src itr_tgt
@@ -265,12 +264,12 @@ Section KSIM.
               (_sim_knot thsl thsr tid rs_local true f_tgt
                          (sf, ktr_src tt)
                          itr_tgt
-                         (im_src0, im_tgt, st_src, st_tgt, o0, r_kshared)))
+                         (im_src0, im_tgt, st_src, st_tgt, r_kshared) o0))
       :
       __sim_knot RR sim_knot _sim_knot thsl thsr tid rs_local f_src f_tgt
                  (sf, Vis (inl1 (inl1 (Fair fm))) ktr_src)
                  (itr_tgt)
-                 (im_src, im_tgt, st_src, st_tgt, o, r_kshared)
+                 (im_src, im_tgt, st_src, st_tgt, r_kshared) o
 
     | ksim_tauR
         tid f_src f_tgt
@@ -280,12 +279,12 @@ Section KSIM.
         (KSIM: _sim_knot thsl thsr tid rs_local f_src true
                          (sf, itr_src)
                          itr_tgt
-                         (im_src, im_tgt, st_src, st_tgt, o, r_kshared))
+                         (im_src, im_tgt, st_src, st_tgt, r_kshared) o)
       :
       __sim_knot RR sim_knot _sim_knot thsl thsr tid rs_local f_src f_tgt
                  (sf, itr_src)
                  (Tau itr_tgt)
-                 (im_src, im_tgt, st_src, st_tgt, o, r_kshared)
+                 (im_src, im_tgt, st_src, st_tgt, r_kshared) o
     | ksim_chooseR
         tid f_src f_tgt
         sf itr_src X ktr_tgt
@@ -294,12 +293,12 @@ Section KSIM.
         (KSIM: forall x, _sim_knot thsl thsr tid rs_local f_src true
                               (sf, itr_src)
                               (ktr_tgt x)
-                              (im_src, im_tgt, st_src, st_tgt, o, r_kshared))
+                              (im_src, im_tgt, st_src, st_tgt, r_kshared) o)
       :
       __sim_knot RR sim_knot _sim_knot thsl thsr tid rs_local f_src f_tgt
                  (sf, itr_src)
                  (Vis (inl1 (inl1 (Choose X))) ktr_tgt)
-                 (im_src, im_tgt, st_src, st_tgt, o, r_kshared)
+                 (im_src, im_tgt, st_src, st_tgt, r_kshared) o
     | ksim_putR
         tid f_src f_tgt
         sf itr_src st_tgt0 ktr_tgt
@@ -308,12 +307,12 @@ Section KSIM.
         (KSIM: _sim_knot thsl thsr tid rs_local f_src true
                          (sf, itr_src)
                          (ktr_tgt tt)
-                         (im_src, im_tgt, st_src, st_tgt0, o, r_kshared))
+                         (im_src, im_tgt, st_src, st_tgt0, r_kshared) o)
       :
       __sim_knot RR sim_knot _sim_knot thsl thsr tid rs_local f_src f_tgt
                  (sf, itr_src)
                  (Vis (inr1 (Mod.Put st_tgt0)) ktr_tgt)
-                 (im_src, im_tgt, st_src, st_tgt, o, r_kshared)
+                 (im_src, im_tgt, st_src, st_tgt, r_kshared) o
     | ksim_getR
         tid f_src f_tgt
         sf itr_src ktr_tgt
@@ -322,12 +321,12 @@ Section KSIM.
         (KSIM: _sim_knot thsl thsr tid rs_local f_src true
                          (sf, itr_src)
                          (ktr_tgt st_tgt)
-                         (im_src, im_tgt, st_src, st_tgt, o, r_kshared))
+                         (im_src, im_tgt, st_src, st_tgt, r_kshared) o)
       :
       __sim_knot RR sim_knot _sim_knot thsl thsr tid rs_local f_src f_tgt
                  (sf, itr_src)
                  (Vis (inr1 (@Mod.Get _)) ktr_tgt)
-                 (im_src, im_tgt, st_src, st_tgt, o, r_kshared)
+                 (im_src, im_tgt, st_src, st_tgt, r_kshared) o
     | ksim_tidR
         tid f_src f_tgt
         sf itr_src ktr_tgt
@@ -336,12 +335,12 @@ Section KSIM.
         (KSIM: _sim_knot thsl thsr tid rs_local f_src true
                          (sf, itr_src)
                          (ktr_tgt tid)
-                         (im_src, im_tgt, st_src, st_tgt, o, r_kshared))
+                         (im_src, im_tgt, st_src, st_tgt, r_kshared) o)
       :
       __sim_knot RR sim_knot _sim_knot thsl thsr tid rs_local f_src f_tgt
                  (sf, itr_src)
                  (Vis (inl1 (inr1 GetTid)) ktr_tgt)
-                 (im_src, im_tgt, st_src, st_tgt, o, r_kshared)
+                 (im_src, im_tgt, st_src, st_tgt, r_kshared) o
     | ksim_fairR
         tid f_src f_tgt
         sf itr_src fm ktr_tgt
@@ -351,12 +350,12 @@ Section KSIM.
             (_sim_knot thsl thsr tid rs_local f_src true
                        (sf, itr_src)
                        (ktr_tgt tt)
-                       (im_src, im_tgt0, st_src, st_tgt, o, r_kshared)))
+                       (im_src, im_tgt0, st_src, st_tgt, r_kshared) o))
       :
       __sim_knot RR sim_knot _sim_knot thsl thsr tid rs_local f_src f_tgt
                  (sf, itr_src)
                  (Vis (inl1 (inl1 (Fair fm))) ktr_tgt)
-                 (im_src, im_tgt, st_src, st_tgt, o, r_kshared)
+                 (im_src, im_tgt, st_src, st_tgt, r_kshared) o
 
     | ksim_observe
         tid f_src f_tgt
@@ -366,12 +365,12 @@ Section KSIM.
         (KSIM: forall ret, sim_knot thsl thsr tid rs_local true true
                                (sf, ktr_src ret)
                                (ktr_tgt ret)
-                               (im_src, im_tgt, st_src, st_tgt, o0, r_kshared))
+                               (im_src, im_tgt, st_src, st_tgt, r_kshared) o0)
       :
       __sim_knot RR sim_knot _sim_knot thsl thsr tid rs_local f_src f_tgt
                  (sf, Vis (inl1 (inl1 (Observe fn args))) ktr_src)
                  (Vis (inl1 (inl1 (Observe fn args))) ktr_tgt)
-                 (im_src, im_tgt, st_src, st_tgt, o, r_kshared)
+                 (im_src, im_tgt, st_src, st_tgt, r_kshared) o
 
     | ksim_progress
         tid
@@ -381,21 +380,21 @@ Section KSIM.
         (KSIM: sim_knot thsl thsr tid rs_local false false
                         (sf, itr_src)
                         itr_tgt
-                        (im_src, im_tgt, st_src, st_tgt, o0, r_kshared))
+                        (im_src, im_tgt, st_src, st_tgt, r_kshared) o0)
       :
       __sim_knot RR sim_knot _sim_knot thsl thsr tid rs_local true true
                  (sf, itr_src)
                  (itr_tgt)
-                 (im_src, im_tgt, st_src, st_tgt, o, r_kshared)
+                 (im_src, im_tgt, st_src, st_tgt, r_kshared) o
   .
 
   Definition sim_knot R0 R1 (RR: R0 -> R1 -> Prop):
     threads_src2 R0 -> threads_tgt R1 -> thread_id -> local_resources ->
-    bool -> bool -> (prod bool (itree srcE R0)) -> (itree tgtE R1) -> kshared -> Prop :=
-    paco9 (fun r => pind9 (__sim_knot RR r) top9) bot9.
+    bool -> bool -> (prod bool (itree srcE R0)) -> (itree tgtE R1) -> kshared -> wf_stt.(T) -> Prop :=
+    paco10 (fun r => pind10 (__sim_knot RR r) top10) bot10.
 
   Lemma __ksim_mon R0 R1 (RR: R0 -> R1 -> Prop):
-    forall r r' (LE: r <9= r'), (__sim_knot RR r) <10= (__sim_knot RR r').
+    forall r r' (LE: r <10= r'), (__sim_knot RR r) <11= (__sim_knot RR r').
   Proof.
     ii. inv PR; try (econs; eauto; fail).
     { econs 2; eauto. i. specialize (KSIM tid0). des; eauto. right.
@@ -409,7 +408,7 @@ Section KSIM.
     }
   Qed.
 
-  Lemma _ksim_mon R0 R1 (RR: R0 -> R1 -> Prop): forall r, monotone9 (__sim_knot RR r).
+  Lemma _ksim_mon R0 R1 (RR: R0 -> R1 -> Prop): forall r, monotone10 (__sim_knot RR r).
   Proof.
     ii. inv IN; try (econs; eauto; fail).
     { des. econs; eauto. }
@@ -417,9 +416,9 @@ Section KSIM.
     { des. econs; eauto. }
   Qed.
 
-  Lemma ksim_mon R0 R1 (RR: R0 -> R1 -> Prop): forall q, monotone9 (fun r => pind9 (__sim_knot RR r) q).
+  Lemma ksim_mon R0 R1 (RR: R0 -> R1 -> Prop): forall q, monotone10 (fun r => pind10 (__sim_knot RR r) q).
   Proof.
-    ii. eapply pind9_mon_gen; eauto.
+    ii. eapply pind10_mon_gen; eauto.
     ii. eapply __ksim_mon; eauto.
   Qed.
 
@@ -432,101 +431,101 @@ Section KSIM.
   Lemma ksim_reset_prog
         R0 R1 (RR: R0 -> R1 -> Prop)
         ths_src ths_tgt tid rs_local
-        ssrc tgt shr
+        ssrc tgt shr o
         ps0 pt0 ps1 pt1
-        (KSIM: sim_knot RR ths_src ths_tgt tid rs_local ps1 pt1 ssrc tgt shr)
+        (KSIM: sim_knot RR ths_src ths_tgt tid rs_local ps1 pt1 ssrc tgt shr o)
         (SRC: ps1 = true -> ps0 = true)
         (TGT: pt1 = true -> pt0 = true)
     :
-    sim_knot RR ths_src ths_tgt tid rs_local ps0 pt0 ssrc tgt shr.
+    sim_knot RR ths_src ths_tgt tid rs_local ps0 pt0 ssrc tgt shr o.
   Proof.
     revert_until RR. pcofix CIH. i.
     move KSIM before CIH. revert_until KSIM. punfold KSIM.
-    pattern ths_src, ths_tgt, tid, rs_local, ps1, pt1, ssrc, tgt, shr.
-    revert ths_src ths_tgt tid rs_local ps1 pt1 ssrc tgt shr KSIM.
-    eapply pind9_acc.
-    intros rr DEC IH ths_src ths_tgt tid rs_local ps1 pt1 ssrc tgt shr KSIM. clear DEC.
+    pattern ths_src, ths_tgt, tid, rs_local, ps1, pt1, ssrc, tgt, shr, o.
+    revert ths_src ths_tgt tid rs_local ps1 pt1 ssrc tgt shr o KSIM.
+    eapply pind10_acc.
+    intros rr DEC IH ths_src ths_tgt tid rs_local ps1 pt1 ssrc tgt shr o KSIM. clear DEC.
     intros ps0 pt0 SRC TGT.
-    eapply pind9_unfold in KSIM.
+    eapply pind10_unfold in KSIM.
     2:{ eapply _ksim_mon. }
     inv KSIM.
 
-    { pfold. eapply pind9_fold. econs; eauto. }
+    { pfold. eapply pind10_fold. econs; eauto. }
 
-    { clear rr IH. pfold. eapply pind9_fold. eapply ksim_ret_cont; eauto. i.
+    { clear rr IH. pfold. eapply pind10_fold. eapply ksim_ret_cont; eauto. i.
       specialize (KSIM0 tid0). des; eauto. right.
       esplits; eauto.
-      - i; hexploit KSIM2; clear KSIM2 KSIM3; eauto. i. eapply upaco9_mon_bot; eauto.
-      - i; hexploit KSIM3; clear KSIM2 KSIM3; eauto. i. des. esplits; eauto. i. eapply upaco9_mon_bot; eauto.
+      - i; hexploit KSIM2; clear KSIM2 KSIM3; eauto. i. eapply upaco10_mon_bot; eauto.
+      - i; hexploit KSIM3; clear KSIM2 KSIM3; eauto. i. des. esplits; eauto. i. eapply upaco10_mon_bot; eauto.
     }
 
-    { clear rr IH. pfold. eapply pind9_fold. eapply ksim_sync; eauto. i.
+    { clear rr IH. pfold. eapply pind10_fold. eapply ksim_sync; eauto. i.
       specialize (KSIM0 tid0). des; eauto. right.
       esplits; eauto.
-      - i; hexploit KSIM2; clear KSIM2 KSIM3; eauto. i. des. esplits; eauto. i. eapply upaco9_mon_bot; eauto.
-      - i; hexploit KSIM3; clear KSIM2 KSIM3; eauto. i. des. esplits; eauto. i. eapply upaco9_mon_bot; eauto.
+      - i; hexploit KSIM2; clear KSIM2 KSIM3; eauto. i. des. esplits; eauto. i. eapply upaco10_mon_bot; eauto.
+      - i; hexploit KSIM3; clear KSIM2 KSIM3; eauto. i. des. esplits; eauto. i. eapply upaco10_mon_bot; eauto.
     }
 
-    { des. pfold. eapply pind9_fold. eapply ksim_yieldL. esplits; eauto. split; ss.
+    { des. pfold. eapply pind10_fold. eapply ksim_yieldL. esplits; eauto. split; ss.
       destruct KSIM1 as [KSIM1 IND]. hexploit IH; eauto. i. punfold H.
     }
 
-    { pfold. eapply pind9_fold. eapply ksim_tauL. split; ss.
+    { pfold. eapply pind10_fold. eapply ksim_tauL. split; ss.
       destruct KSIM0 as [KSIM0 IND]. hexploit IH; eauto. i. punfold H.
     }
 
-    { des. pfold. eapply pind9_fold. eapply ksim_chooseL. esplits. split; ss.
+    { des. pfold. eapply pind10_fold. eapply ksim_chooseL. esplits. split; ss.
       destruct KSIM0 as [KSIM0 IND]. hexploit IH; eauto. i. punfold H.
     }
 
-    { pfold. eapply pind9_fold. eapply ksim_putL. split; ss.
+    { pfold. eapply pind10_fold. eapply ksim_putL. split; ss.
       destruct KSIM0 as [KSIM0 IND]. hexploit IH; eauto. i. punfold H.
     }
 
-    { pfold. eapply pind9_fold. eapply ksim_getL. split; ss.
+    { pfold. eapply pind10_fold. eapply ksim_getL. split; ss.
       destruct KSIM0 as [KSIM0 IND]. hexploit IH; eauto. i. punfold H.
     }
 
-    { pfold. eapply pind9_fold. eapply ksim_tidL. split; ss.
+    { pfold. eapply pind10_fold. eapply ksim_tidL. split; ss.
       destruct KSIM0 as [KSIM0 IND]. hexploit IH; eauto. i. punfold H.
     }
 
-    { pfold. eapply pind9_fold. eapply ksim_UB. }
+    { pfold. eapply pind10_fold. eapply ksim_UB. }
 
-    { des. pfold. eapply pind9_fold. eapply ksim_fairL. esplits; eauto. split; ss.
+    { des. pfold. eapply pind10_fold. eapply ksim_fairL. esplits; eauto. split; ss.
       destruct KSIM1 as [KSIM1 IND]. hexploit IH; eauto. i. punfold H.
     }
 
-    { pfold. eapply pind9_fold. eapply ksim_tauR. split; ss.
+    { pfold. eapply pind10_fold. eapply ksim_tauR. split; ss.
       destruct KSIM0 as [KSIM0 IND]. hexploit IH; eauto. i. punfold H.
     }
 
-    { pfold. eapply pind9_fold. eapply ksim_chooseR. i. split; ss. specialize (KSIM0 x).
+    { pfold. eapply pind10_fold. eapply ksim_chooseR. i. split; ss. specialize (KSIM0 x).
       destruct KSIM0 as [KSIM0 IND]. hexploit IH; eauto. i. punfold H.
     }
 
-    { pfold. eapply pind9_fold. eapply ksim_putR. split; ss.
+    { pfold. eapply pind10_fold. eapply ksim_putR. split; ss.
       destruct KSIM0 as [KSIM0 IND]. hexploit IH; eauto. i. punfold H.
     }
 
-    { pfold. eapply pind9_fold. eapply ksim_getR. split; ss.
+    { pfold. eapply pind10_fold. eapply ksim_getR. split; ss.
       destruct KSIM0 as [KSIM0 IND]. hexploit IH; eauto. i. punfold H.
     }
 
-    { pfold. eapply pind9_fold. eapply ksim_tidR. split; ss.
+    { pfold. eapply pind10_fold. eapply ksim_tidR. split; ss.
       destruct KSIM0 as [KSIM0 IND]. hexploit IH; eauto. i. punfold H.
     }
 
-    { pfold. eapply pind9_fold. eapply ksim_fairR. i. split; ss. specialize (KSIM0 _ FAIR).
+    { pfold. eapply pind10_fold. eapply ksim_fairR. i. split; ss. specialize (KSIM0 _ FAIR).
       destruct KSIM0 as [KSIM0 IND]. hexploit IH; eauto. i. punfold H.
     }
 
-    { pfold. eapply pind9_fold. eapply ksim_observe. i. specialize (KSIM0 ret). pclearbot.
+    { pfold. eapply pind10_fold. eapply ksim_observe. i. specialize (KSIM0 ret). pclearbot.
       right; eapply CIH; eauto.
     }
 
     { hexploit SRC; ss; i; clarify. hexploit TGT; ss; i; clarify.
-      pfold. eapply pind9_fold. eapply ksim_progress. pclearbot.
+      pfold. eapply pind10_fold. eapply ksim_progress. pclearbot.
       right; eapply CIH; eauto.
     }
 
@@ -545,91 +544,91 @@ Section KSIM.
   (*   move KSIM before CIH. revert_until KSIM. punfold KSIM. *)
   (*   pattern ths_src, ths_tgt, tid, rs_local, ps1, pt1, ssrc, tgt, shr. *)
   (*   revert ths_src ths_tgt tid rs_local ps1 pt1 ssrc tgt shr KSIM. *)
-  (*   eapply pind9_acc. *)
+  (*   eapply pind10_acc. *)
   (*   intros rr DEC IH ths_src ths_tgt tid rs_local ps1 pt1 ssrc tgt shr KSIM. clear DEC. *)
   (*   intros Eps1 Ept1 ps pt. clarify. *)
-  (*   eapply pind9_unfold in KSIM. *)
+  (*   eapply pind10_unfold in KSIM. *)
   (*   2:{ eapply _ksim_mon. } *)
   (*   inv KSIM. *)
 
-  (*   { pfold. eapply pind9_fold. econs; eauto. } *)
+  (*   { pfold. eapply pind10_fold. econs; eauto. } *)
 
-  (*   { clear rr IH. pfold. eapply pind9_fold. eapply ksim_ret_cont; eauto. i. *)
+  (*   { clear rr IH. pfold. eapply pind10_fold. eapply ksim_ret_cont; eauto. i. *)
   (*     specialize (KSIM0 tid0). des; eauto. right. *)
   (*     esplits; eauto. *)
-  (*     - i; hexploit KSIM2; clear KSIM2 KSIM3; eauto. i. eapply upaco9_mon_bot; eauto. *)
+  (*     - i; hexploit KSIM2; clear KSIM2 KSIM3; eauto. i. eapply upaco10_mon_bot; eauto. *)
   (*     - i; hexploit KSIM3; clear KSIM2 KSIM3; eauto. i. des. esplits; eauto. *)
-  (*       i. eapply upaco9_mon_bot; eauto. *)
+  (*       i. eapply upaco10_mon_bot; eauto. *)
   (*   } *)
 
-  (*   { clear rr IH. pfold. eapply pind9_fold. eapply ksim_sync; eauto. i. *)
+  (*   { clear rr IH. pfold. eapply pind10_fold. eapply ksim_sync; eauto. i. *)
   (*     specialize (KSIM0 tid0). des; eauto. right. *)
   (*     esplits; eauto. *)
-  (*     - i; hexploit KSIM2; clear KSIM2 KSIM3; eauto. i. des. esplits; eauto. i. eapply upaco9_mon_bot; eauto. *)
-  (*     - i; hexploit KSIM3; clear KSIM2 KSIM3; eauto. i. des. esplits; eauto. i. eapply upaco9_mon_bot; eauto. *)
+  (*     - i; hexploit KSIM2; clear KSIM2 KSIM3; eauto. i. des. esplits; eauto. i. eapply upaco10_mon_bot; eauto. *)
+  (*     - i; hexploit KSIM3; clear KSIM2 KSIM3; eauto. i. des. esplits; eauto. i. eapply upaco10_mon_bot; eauto. *)
   (*   } *)
 
-  (*   { des. pfold. eapply pind9_fold. eapply ksim_yieldL. esplits; eauto. split; ss. *)
+  (*   { des. pfold. eapply pind10_fold. eapply ksim_yieldL. esplits; eauto. split; ss. *)
   (*     destruct KSIM1 as [KSIM1 IND]. hexploit IH; eauto. i. punfold H. *)
   (*   } *)
 
-  (*   { pfold. eapply pind9_fold. eapply ksim_tauL. split; ss. *)
+  (*   { pfold. eapply pind10_fold. eapply ksim_tauL. split; ss. *)
   (*     destruct KSIM0 as [KSIM0 IND]. hexploit IH; eauto. i. punfold H. *)
   (*   } *)
 
-  (*   { des. pfold. eapply pind9_fold. eapply ksim_chooseL. esplits. split; ss. *)
+  (*   { des. pfold. eapply pind10_fold. eapply ksim_chooseL. esplits. split; ss. *)
   (*     destruct KSIM0 as [KSIM0 IND]. hexploit IH; eauto. i. punfold H. *)
   (*   } *)
 
-  (*   { pfold. eapply pind9_fold. eapply ksim_putL. split; ss. *)
+  (*   { pfold. eapply pind10_fold. eapply ksim_putL. split; ss. *)
   (*     destruct KSIM0 as [KSIM0 IND]. hexploit IH; eauto. i. punfold H. *)
   (*   } *)
 
-  (*   { pfold. eapply pind9_fold. eapply ksim_getL. split; ss. *)
+  (*   { pfold. eapply pind10_fold. eapply ksim_getL. split; ss. *)
   (*     destruct KSIM0 as [KSIM0 IND]. hexploit IH; eauto. i. punfold H. *)
   (*   } *)
 
-  (*   { pfold. eapply pind9_fold. eapply ksim_tidL. split; ss. *)
+  (*   { pfold. eapply pind10_fold. eapply ksim_tidL. split; ss. *)
   (*     destruct KSIM0 as [KSIM0 IND]. hexploit IH; eauto. i. punfold H. *)
   (*   } *)
 
-  (*   { pfold. eapply pind9_fold. eapply ksim_UB. } *)
+  (*   { pfold. eapply pind10_fold. eapply ksim_UB. } *)
 
-  (*   { des. pfold. eapply pind9_fold. eapply ksim_fairL. esplits; eauto. split; ss. *)
+  (*   { des. pfold. eapply pind10_fold. eapply ksim_fairL. esplits; eauto. split; ss. *)
   (*     destruct KSIM1 as [KSIM1 IND]. hexploit IH; eauto. i. punfold H. *)
   (*   } *)
 
-  (*   { pfold. eapply pind9_fold. eapply ksim_tauR. split; ss. *)
+  (*   { pfold. eapply pind10_fold. eapply ksim_tauR. split; ss. *)
   (*     destruct KSIM0 as [KSIM0 IND]. hexploit IH; eauto. i. punfold H. *)
   (*   } *)
 
-  (*   { pfold. eapply pind9_fold. eapply ksim_chooseR. i. split; ss. specialize (KSIM0 x). *)
+  (*   { pfold. eapply pind10_fold. eapply ksim_chooseR. i. split; ss. specialize (KSIM0 x). *)
   (*     destruct KSIM0 as [KSIM0 IND]. hexploit IH; eauto. i. punfold H. *)
   (*   } *)
 
-  (*   { pfold. eapply pind9_fold. eapply ksim_putR. split; ss. *)
+  (*   { pfold. eapply pind10_fold. eapply ksim_putR. split; ss. *)
   (*     destruct KSIM0 as [KSIM0 IND]. hexploit IH; eauto. i. punfold H. *)
   (*   } *)
 
-  (*   { pfold. eapply pind9_fold. eapply ksim_getR. split; ss. *)
+  (*   { pfold. eapply pind10_fold. eapply ksim_getR. split; ss. *)
   (*     destruct KSIM0 as [KSIM0 IND]. hexploit IH; eauto. i. punfold H. *)
   (*   } *)
 
-  (*   { pfold. eapply pind9_fold. eapply ksim_tidR. split; ss. *)
+  (*   { pfold. eapply pind10_fold. eapply ksim_tidR. split; ss. *)
   (*     destruct KSIM0 as [KSIM0 IND]. hexploit IH; eauto. i. punfold H. *)
   (*   } *)
 
-  (*   { pfold. eapply pind9_fold. eapply ksim_fairR. i. split; ss. specialize (KSIM0 _ FAIR). *)
+  (*   { pfold. eapply pind10_fold. eapply ksim_fairR. i. split; ss. specialize (KSIM0 _ FAIR). *)
   (*     destruct KSIM0 as [KSIM0 IND]. hexploit IH; eauto. i. punfold H. *)
   (*   } *)
 
-  (*   { pfold. eapply pind9_fold. eapply ksim_observe. i. specialize (KSIM0 ret). pclearbot. *)
+  (*   { pfold. eapply pind10_fold. eapply ksim_observe. i. specialize (KSIM0 ret). pclearbot. *)
   (*     right; eapply CIH; eauto. *)
   (*   } *)
 
-  (*   { pclearbot. pfold. eapply pind9_fold. eapply ksim_progress.  *)
+  (*   { pclearbot. pfold. eapply pind10_fold. eapply ksim_progress.  *)
 
-  (*     eapply paco9_mon_bot; eauto. eapply ksim_reset_prog. eauto. all: auto. } *)
+  (*     eapply paco10_mon_bot; eauto. eapply ksim_reset_prog. eauto. all: auto. } *)
 
   (* Qed. *)
 
